src/Lib/Chloe_Base.thy
@@ -4,6 +4,7 @@ imports
   "~~/src/HOL/Library/Code_Target_Int"
   "~~/src/HOL/Library/Code_Target_Nat"
   "Native_Word/Code_Target_Bits_Int"
+  Chloe_Misc
   Chloe_Monad Lenses Gen_Cases
 begin
 
